linkedListSearch and bubble sort

bubblesort/bubblesort.dfy
@@ -1,59 +1,54 @@
-predicate IsSorted(arr: array<int>) {
-  forall i, j :: 0 <= i <= j < arr.Length ==> arr[i] <= arr[j]
+predicate Sorted(s: seq<int>)
+{
+  forall i, j :: 0 <= i < j < |s| ==> s[i] <= s[j]
 }
 
-method BubbleSort(arr: array<int>)
-  modifies arr
-  ensures IsSorted(arr)
+predicate Partitioned(s: seq<int>, k: int)
 {
-  var n := arr.Length;
-  var pass := 0;
-  while pass < n
-    invariant 0 <= pass <= n
+  0 <= k <= |s| &&
+  (forall p, q :: 0 <= p < k && k <= q < |s| ==> s[p] <= s[q])
+}
+
+method BubbleSort(a: array<int>)
+  modifies a
+  ensures Sorted(a[..])
+{
+  var n := a.Length;
+  if n <= 1 { return; }
+
+  var i := 0;
+  while i < n
+    invariant 0 <= i <= n
+    invariant Sorted(a[n - i .. n]) // a[n-i]...a[n-1] are sorted
+    invariant Partitioned(a[..], n - i) // each element in a[0]...a[n-i-1] is smaller than each element in a[n-i]...a[n-1]
   {
-    var j := 0;
-    while j < n - 1 {
-      if arr[j] > arr[j + 1] {
-        var temp := arr[j];
-        arr[j] := arr[j + 1];
-        arr[j + 1] := temp;
+    var j := 1;
+    while j < n - i
+      invariant 1 <= j <= n - i
+      invariant Sorted(a[n - i .. n]) // keep invariant
+      invariant Partitioned(a[..], n - i) // keep invariant
+      invariant forall k :: 0 <= k < j ==> a[k] <= a[j - 1] // a[j-1] is maximal among a[0]...a[j-1]
+    {
+      if a[j - 1] > a[j] {
+        var t := a[j - 1];
+        a[j - 1] := a[j];
+        a[j] := t;
       }
       j := j + 1;
     }
-    pass := pass + 1;
+    i := i + 1;
   }
 }
 
-method Main(args: seq<string>) {
-  print("Bubble sort example:\n");
+method Main()
+{
+  var s := [5, 1, 4, 2, 8, 0, 1 ,1, 7];
+  
+  // array initialization surely not optimal 
+  var a := new int[|s|] (i => 0); 
+  for i := 0 to |s| { a[i] := s[i]; }
 
-  var arr := new int[5];
-  arr[0] := 64;
-  arr[1] := 34;
-  arr[2] := 25;
-  arr[3] := 12;
-  arr[4] := 22;
-
-  print("Original array: ");
-  var i := 0;
-  while i < arr.Length {
-    print(arr[i]);
-    print(" ");
-    i := i + 1;
-  }
-  print("\n");
-
-  BubbleSort(arr);
-
-  print("Sorted array: ");
-  i := 0;
-  while i < arr.Length {
-    print(arr[i]);
-    print(" ");
-    i := i + 1;
-  }
-  print("\n");
-
-  assert IsSorted(arr);
-  print("✓ Array is correctly sorted!\n");
+  print a[..], "\n"; 
+  BubbleSort(a);
+  print a[..], "\n"; 
 }
